Added support for shared references to ghostseq and permdata and GhostPtrToken borrow to use it

theories/typing/lib/ghostptrtoken/ghostptrtoken_index.v
@@ -6,30 +6,7 @@ Set Default Proof Using "Type".
 Open Scope nat.
 Implicit Type 𝔄 𝔅: syn_type.
 
-Section ghostptrtoken_insertremove.
-  Context `{!typeG Σ}.
-
-  Definition ghostptrtoken_insert {𝔄} (ty: type 𝔄) : val :=
-    fn: ["t"; "b"] :=
-      Skip;;
-      delete [ #1; "t"];;
-      return: ["b"].
-
-  Lemma ghostptrtoken_insert_type {𝔄} (ty: type 𝔄) :
-   (ty.(ty_size) > 0) → typed_val (ghostptrtoken_insert ty) (fn<α>(∅; &uniq{α} (ghostptrtoken_ty ty), box ty) → ptr)
-      (λ post '-[(al, al'); a], forall ptr, (list_to_gmap al') = <[ptr:=a]>(list_to_gmap al) → (list_to_gmap al) !! ptr = None → post ptr).
-  Proof.
-    intros ?. eapply type_fn; [apply _|]=> α ??[l[l2[]]]. simpl_subst. via_tr_impl.
-    iApply ghost_read_delete; [done|]. iIntros. iApply typed_body_tctx_incl.
-    eapply ghost_update; [done|solve_typing|]. 
-    eapply tctx_incl_trans. eapply (tctx_incl_frame_l _ _ +[_]). eapply tctx_incl_trans. eapply permdata_from_box. eapply tctx_incl_swap.
-    simpl. eapply (tctx_incl_frame_r +[_; _] +[_] +[_]). eapply seq_cons. done.
-    iApply type_jump; [solve_typing|solve_extract|].
-    apply resolve_tctx_cons_hasty. eapply uniq_resolve'; [eapply always_true_ghostptrtoken_nodup'; lia|solve_typing]. apply resolve_tctx_nil.
-    move=>post [[tc tf][v []]]Impl l' [eq nodup]/=. rewrite eq in Impl. apply Impl. done.
-    apply not_elem_of_list_to_map_1. inversion_clear nodup. done.
-  Qed.
-
+Section index.
   Definition find_idx {A} P `{∀ x, Decision (P x)} : list A → nat :=
     fix go l :=
     match l with
@@ -95,7 +72,10 @@ Section ghostptrtoken_insertremove.
     inversion_clear no_dup. destruct (decide (a0.1 = k)) as [<-|]; simpl. done.
     apply not_elem_of_cons. split. done. apply IHl. done.
   Qed.
+End index.
 
+Section find_logic.
+  Context `{!typeG Σ}.
   Lemma find_logic {𝔄 𝔄'} (ty: type (𝔄*𝔄')) (ty': plain_type 𝔄) `{!EqDecision 𝔄} :
     (∀ vπ ξl, ty_proph ty vπ ξl → ∃ (x: 𝔄) (vπ': proph 𝔄'), vπ = (λ π, (x, vπ' π))) → logic_fn +[ghostseq.ghostseq_ty ty; (ty': type 𝔄)] int (λ '-[l; k], find_idx (λ (x: (𝔄*𝔄')) , x.1 = k) l).
   Proof. intros ? (?&?&[]) ((?&?&?&->&->&?)&(?&?&->)&[]). exists [].
@@ -104,6 +84,44 @@ Section ghostptrtoken_insertremove.
     destruct (IHrest x1 H2) as (res&eq). exists (Z.succ res). fun_ext=>π/=. specialize (equal_f eq π)=>/=<-. lia.
   Qed.
 
+  Lemma find_permdata_logic {𝔄} (ty: type 𝔄) :
+    logic_fn +[ghostptrtoken_ty ty; ptr] int (λ '-[l; k], find_idx (λ x , x.1 = k) l).
+  Proof. apply find_logic. intros ??(?&?&->&?). eexists _, _. done. Qed.
+End find_logic.
+
+Section ghostptrtoken_borrow.
+  Context `{!typeG Σ}.
+
+  Definition ghostptrtoken_borrow {𝔄} (ty: type 𝔄) : val :=
+    fn: ["t"; "p"] :=
+      Skip;;
+      delete [ #1; "t"];;
+      (Skip;;Skip);;
+      (Skip;;Skip);;
+      return: ["p"].
+
+  (* Rust's GhostPtrToken::borrow_mut *)
+  Lemma ghostptrtoken_borrow_type {𝔄} (ty: type 𝔄):
+    typed_val (ghostptrtoken_borrow ty) (fn<α>(∅; &shr{α} (ghostptrtoken_ty ty), ptr) → &shr{α} ty)
+      (λ post '-[l; ptr], exists v, (list_to_gmap l) !! ptr = Some(v) ∧ post (v)).
+  Proof.
+    fold of_syn_type. eapply type_fn; [apply _|]=> ???[ol[pl[]]]. simpl_subst. via_tr_impl.
+    iApply ghost_read_delete. done. iIntros (?).
+    iApply ghost_new; [solve_typing|].
+    iApply typed_body_tctx_incl. eapply tctx_incl_trans. eapply tctx_incl_tail. apply tctx_incl_swap. apply tctx_incl_swap.
+    iApply ghost_new; [solve_typing|].
+    iApply typed_body_tctx_incl. eapply tctx_incl_trans. eapply tctx_incl_swap. eapply tctx_incl_trans. eapply tctx_incl_tail. 
+    eapply tctx_incl_trans. eapply (tctx_incl_frame_r +[_; _]). eapply tctx_incl_trans. eapply tctx_incl_tail. eapply (logic_fn_ghost_tctx_incl' [_] _ +[]). apply shr_deref_logic_fn.
+    eapply tctx_incl_trans. apply tctx_incl_swap. eapply (logic_fn_ghost_tctx_incl' [_; _] _ +[_]).
+    apply find_permdata_logic. eapply tctx_incl_trans. eapply tctx_incl_swap. apply seq_shr_index. done. eapply permdata_shr.
+    iApply type_jump; [solve_typing|solve_extract|solve_typing].
+    rewrite /trans_upper /trans_tail. move=>post [s[l []]][v [lookup ?]]. simpl.
+    eexists _, _. destruct (find_idx_delete _ _ _ lookup). intuition. rewrite H0. done. done.
+  Qed.
+End ghostptrtoken_borrow.
+
+Section ghostptrtoken_insertremove.
+  Context `{!typeG Σ}.
 
   Definition ghostptrtoken_remove {𝔄} (ty: type 𝔄) : val :=
     fn: ["t"; "ptr"] :=
